chg: Rearrangements in Casari.v !minor

theories/FO/Casari.v
@@ -1,42 +1,8 @@
 From InqLog Require Export Truth.
 
-(** * Example signature *)
-
-Instance signature : Signature :=
-  {|
-    PSymb := unit;
-    PAri := fun p => match p with tt => unit end;
-    FSymb := Empty_set;
-    FAri := fun f => match f with end;
-    rigid := fun _ => true
-  |}.
-
-Definition Pred' (t : term) := Pred tt (fun arg => t).
-
-Theorem CasariProp (P : var -> Prop) :
-  (
-    forall x,
-      (
-        (P x)
-        ->
-        (forall x, ~ ~ P x)
-      )
-      ->
-      (forall x, ~ ~ P x)
-  )
-  ->
-  (
-    forall x, ~ ~ P x
-  ).
-Proof.
-  firstorder.
-Qed.
-
-Print Assumptions CasariProp.
-
 (** * Casari Scheme *)
 
-Definition Casari (phi : var -> form) : form :=
+Definition Casari `{Signature} (phi : var -> form) : form :=
   Impl
   (
     Forall
@@ -60,7 +26,7 @@ Definition Casari (phi : var -> form) : form :=
     Forall (phi 0)
   ).
 
-Theorem Casari_truth_conditional :
+Lemma Casari_truth_conditional `{Signature} :
   forall phi,
     (forall x, classic (phi x) = true) ->
     truth_conditional (Casari phi).
@@ -72,132 +38,166 @@ Proof.
   reflexivity.
 Qed.
 
-(** * Some Casari instances *)
+(** * Some Casari Instances with atomic predicates *)
 
-Definition CasariDNA : form :=
-  Casari (fun x => Neg (Neg (Pred' (Var x)))).
+Module Casari_with_atoms.
 
-Definition CasariAtomic : form :=
-  Casari (fun x => Pred' (Var x)).
+  Instance signature : Signature :=
+    {|
+      PSymb := unit;
+      PAri := fun p => match p with tt => unit end;
+      FSymb := Empty_set;
+      FAri := fun f => match f with end;
+      rigid := fun _ => true
+    |}.
 
-Theorem truth_CasariDNA `{@Model signature} :
-  forall w a,
-    truth CasariDNA w a.
-Proof.
-  intros w1 a.
+  Definition Pred' (t : term) := Pred tt (fun arg => t).
 
-  intros s2 H1 H2.
+  Definition CasariDNA : form :=
+    Casari (fun x => Neg (Neg (Pred' (Var x)))).
 
-  apply substate_singleton in H1 as [H1|H1]; rewrite H1 in *; clear s2 H1.
-  now apply empty_state_property.
+  Definition CasariAtomic : form :=
+    Casari (fun x => Pred' (Var x)).
 
-  intros i1.
-  rewrite support_Neg.
-  intros [s3 [[w2 H3] [H4 H5]]].
-
-  enough (
-    exists s,
-      support (Forall (Neg (Neg (Pred' (Var 0))))) s (i1 .: a) /\
-      substate s3 s
-  ) as [s4 [H6 H7]].
-  {
-    specialize (H6 i1). fold support in H6.
-
-    rewrite support_Neg in H6.
-    apply H6.
-    exists s3.
+  Remark CasariDNA_Prop (P : var -> Prop) :
+    (
+      forall x,
+        (
+          (P x)
+          ->
+          (forall x, ~ ~ P x)
+        )
+        ->
+        (forall x, ~ ~ P x)
+    )
+    ->
+    (
+      forall x, ~ ~ P x
+    ).
+  Proof.
     firstorder.
-  }
+  Qed.
 
-  specialize (H2 i1). fold support in H2.
-  remember (Neg (Neg (Pred' (Var 0)))) as phi1 eqn:eq1.
-  remember (Forall phi1) as phi2 eqn:eq2.
-  remember (Impl phi1 phi2) as phi3 eqn:eq3.
+  Theorem truth_CasariDNA `{@Model signature} :
+    forall w a,
+      truth CasariDNA w a.
+  Proof.
+    intros w1 a.
+
+    intros s2 H1 H2.
+
+    apply substate_singleton in H1 as [H1|H1]; rewrite H1 in *; clear s2 H1.
+    now apply empty_state_property.
+
+    intros i1.
+    rewrite support_Neg.
+    intros [s3 [[w2 H3] [H4 H5]]].
+
+    enough (
+      exists s,
+        support (Forall (Neg (Neg (Pred' (Var 0))))) s (i1 .: a) /\
+        substate s3 s
+    ) as [s4 [H6 H7]].
+    {
+      specialize (H6 i1). fold support in H6.
+
+      rewrite support_Neg in H6.
+      apply H6.
+      exists s3.
+      firstorder.
+    }
+
+    specialize (H2 i1). fold support in H2.
+    remember (Neg (Neg (Pred' (Var 0)))) as phi1 eqn:eq1.
+    remember (Forall phi1) as phi2 eqn:eq2.
+    remember (Impl phi1 phi2) as phi3 eqn:eq3.
 
 
-  eexists.
-  split.
-
-  apply H2. exact H4.
-
-  fold support.
-  subst phi3.
-
-  apply substate_singleton in H4 as [H4|H4]; rewrite H4 in *; clear s3 H4.
-  now apply empty_state_property.
-
-  intros s4 H6 H7.
-
-  apply substate_singleton in H6 as [H6|H6]; rewrite H6 in *; clear s4 H6.
-  now apply empty_state_property.
-
-  exfalso.
-
-  rewrite eq1 in H7.
-  rewrite support_Neg in H7.
-  apply H7.
-
-  eexists.
-  repeat split.
-  -
     eexists.
-    exact H3.
-  -
-    reflexivity.
-  -
-    exact H5.
-  -
-    reflexivity.
-Qed.
+    split.
 
-Corollary support_valid_CasariDNA :
-  support_valid CasariDNA.
-Proof.
-  intros M s a.
-  apply Casari_truth_conditional.
-  -
-    reflexivity.
-  -
-    intros w H1.
-    apply truth_CasariDNA.
-Qed.
+    apply H2. exact H4.
 
-Theorem support_conseq_CasariDNA_CasariAtomic :
-  support_conseq CasariDNA CasariAtomic.
-Proof.
-  unfold CasariDNA.
-  unfold CasariAtomic.
-  unfold Casari.
+    fold support.
+    subst phi3.
 
-  apply support_conseq_Impl.
-  apply support_conseq_Forall.
-  apply support_conseq_Impl.
-  apply support_conseq_Impl.
+    apply substate_singleton in H4 as [H4|H4]; rewrite H4 in *; clear s3 H4.
+    now apply empty_state_property.
 
-  firstorder.
+    intros s4 H6 H7.
 
-  apply support_conseq_Forall.
+    apply substate_singleton in H6 as [H6|H6]; rewrite H6 in *; clear s4 H6.
+    now apply empty_state_property.
 
-  apply support_valid_Impl_conseq.
-  intros *.
-  apply support_valid_DNE_Pred.
+    exfalso.
 
-  apply support_conseq_Forall.
+    rewrite eq1 in H7.
+    rewrite support_Neg in H7.
+    apply H7.
 
-  firstorder.
+    eexists.
+    repeat split.
+    -
+      eexists.
+      exact H3.
+    -
+      reflexivity.
+    -
+      exact H5.
+    -
+      reflexivity.
+  Qed.
 
-  apply support_conseq_Forall.
-  apply support_valid_Impl_conseq.
-  intros *.
-  apply support_valid_DNE_Pred.
-Qed.
+  Corollary support_valid_CasariDNA :
+    support_valid CasariDNA.
+  Proof.
+    intros M s a.
+    apply Casari_truth_conditional.
+    -
+      reflexivity.
+    -
+      intros w H1.
+      apply truth_CasariDNA.
+  Qed.
 
-Corollary support_valid_CasariAtomic :
-  support_valid CasariAtomic.
-Proof.
-  eapply support_valid_conseq_valid.
-  -
-    exact support_valid_CasariDNA.
-  -
-    exact support_conseq_CasariDNA_CasariAtomic.
-Qed.
+  Theorem support_conseq_CasariDNA_CasariAtomic :
+    support_conseq CasariDNA CasariAtomic.
+  Proof.
+    unfold CasariDNA.
+    unfold CasariAtomic.
+    unfold Casari.
+
+    apply support_conseq_Impl.
+    apply support_conseq_Forall.
+    apply support_conseq_Impl.
+    apply support_conseq_Impl.
+
+    firstorder.
+
+    apply support_conseq_Forall.
+
+    apply support_valid_Impl_conseq.
+    intros *.
+    apply support_valid_DNE_Pred.
+
+    apply support_conseq_Forall.
+
+    firstorder.
+
+    apply support_conseq_Forall.
+    apply support_valid_Impl_conseq.
+    intros *.
+    apply support_valid_DNE_Pred.
+  Qed.
+
+  Corollary support_valid_CasariAtomic :
+    support_valid CasariAtomic.
+  Proof.
+    eapply support_valid_conseq_valid.
+    -
+      exact support_valid_CasariDNA.
+    -
+      exact support_conseq_CasariDNA_CasariAtomic.
+  Qed.
+
+End Casari_with_atoms.
